predicate_nnf.v
@@ -1,0 +1,67 @@
+Require Import Formula FindVal OptSolver.
+Require Import Btauto.
+
+
+
+Fixpoint nnf_converter (hn :Datatypes.bool) (p :form) : form :=
+  match hn, p with
+  | false, var _ =>  p
+  | true, var _ => (not  p)
+  | false, boolv _ => p
+  | true, boolv true => boolv false
+  | true, boolv false => boolv true   
+  | false, land p1 p2 => land (nnf_converter false p1) (nnf_converter false p2)
+  | true, land p1 p2 =>  lor (nnf_converter true  p1) (nnf_converter true  p2)
+  | false, lor p1 p2 => lor (nnf_converter false p1) (nnf_converter false p2)
+  | true, lor p1 p2 =>  land (nnf_converter true  p1) (nnf_converter true  p2)
+  | false, mapsto p1 p2 => lor (nnf_converter true p1) (nnf_converter false p2)
+  | true, mapsto p1 p2 => land  (nnf_converter false p1)  (nnf_converter true p2)   
+  | false, not p1  => (nnf_converter true p1)
+  | true, not p1  => (nnf_converter false p1)
+  end.
+
+
+
+(** Check formula is in NNF form. *)
+Inductive is_nnf : form -> Prop :=
+| var : forall i, is_nnf (var i)
+| boolv : forall b, is_nnf (boolv b)
+| land: forall p1 p2, is_nnf p1 -> is_nnf p2 -> is_nnf (land p1 p2)
+| lor: forall p1 p2, is_nnf p1 -> is_nnf p2 -> is_nnf (lor p1 p2)
+| not: forall i, is_nnf (not (var i))
+.
+  
+(** true/false doesn't matter! *)
+(* can't do split at beginning*)
+Lemma is_nnf_neg : forall (p:form), is_nnf (nnf_converter true p) <-> is_nnf (nnf_converter false p).
+  Proof.
+    intros.
+    induction  p;simpl;
+    constructor;intros;
+      try (inversion H; (*land lor mapsto*)
+        apply IHp1 in H2;
+        apply IHp2 in H3;
+        constructor;
+        assumption);
+      try constructor; (*var*)
+      try (apply IHp in H; (*not*)
+        assumption).
+    - destruct b;constructor. (*bool*)
+  Qed.
+  
+    
+(** Conversion is correct. *)
+Lemma nnf_converter_correctness_2: forall (p:form), is_nnf (nnf_converter false  p).
+Proof.
+  intro.
+  induction p;simpl.
+  - constructor.
+  - constructor.
+  - constructor;assumption.
+  - constructor;assumption.
+  - apply is_nnf_neg in IHp1.
+    constructor;assumption.
+  - apply is_nnf_neg.
+    assumption.
+Qed.
+
